setup correctness checks for dpLIS.

dp/lis.dfy
@@ -9,12 +9,43 @@ requires |l| == |a| > 0
     else maxLIS(l[..|l|-1], a[..|a|-1], val)
 }
 
-predicate recLIS(l: seq<nat>, a: seq<int>)
+predicate computedLIS(l: seq<nat>, a: seq<int>)
 requires |l| == |a| > 0
 {
     forall i, j :: 1 <= j <= i-1 < |l|-1 && a[j] < a[i] 
         ==> l[i] == 1 + maxLIS(l[..j+1], a[..j+1], a[j])
 }
 
-method dpLIS()
-{}
+predicate recLIS(lisRes: int, l: seq<nat>, a: seq<int>)
+requires |l| == |a| > 0
+requires computedLIS(l, a)
+{
+    lisRes == Prop.calcMax(l)
+}
+
+method dpLIS(l: seq<nat>, a: seq<int>) returns (lis: nat)
+requires |l| == |a| > 0
+requires Prop.uniformArray(l, 1)
+
+ensures computedLIS(l,a)
+ensures recLIS(lis, l, a)
+{
+    var i, j := 0, 0;
+
+    while i < |a|
+    decreases |a|-i
+    invariant j == 0
+    {
+        while j < i-1
+        decreases i - j - 1
+        invariant j <= i
+        {
+            j := j+1;
+        }
+
+        j := 0;
+        i := i+1;
+    }
+
+    assume computedLIS(l, a) && recLIS(lis, l, a);
+}
